prove Lemma B

botworld_dataScript.sml
@@ -129,7 +129,9 @@ val _ = Parse.type_abbrev("history",``:grid llist``);
 val _ = Parse.type_abbrev("utilityfn",``:history -> real``);
 
 val utilityfn_def = Define`
-  utilityfn (u:utilityfn) ⇔ ∀s h h'. u h ≤ u h' ⇒ u (s ::: h) ≤ u (s ::: h')`;
+  utilityfn (u:utilityfn) ⇔
+    (∀x. 0 ≤ u x ∧ u x ≤ 1) ∧
+    ∀s h h'. u h ≤ u h' ⇒ u (s ::: h) ≤ u (s ::: h')`;
 
 val _ = Datatype`level = MP | Trust num`;
 
